Add .gitignore, Makefile

SAT.v
@@ -1,56 +1,6 @@
-Require Import List Ensembles String Setoid RelationClasses Morphisms Morphisms_Prop Program Equivalence Min Max.
+Require Import List Ensembles String Setoid RelationClasses Morphisms Morphisms_Prop Program Equivalence Min Max Permutation Sorted.
 Require Import JMeq ProofIrrelevance.
-
-Set Implicit Arguments.
-Generalizable All Variables.
-
-Reserved Notation "x >>= y" (at level 42, right associativity).
-Reserved Notation "x <- y ; z" (at level 42, right associativity).
-Reserved Notation "x ;; z" (at level 42, right associativity).
-Reserved Notation "'return' x" (at level 40, no associativity).
-
-Delimit Scope comp_scope with comp.
-
-Ltac apply_in_hyp lem :=
-  match goal with
-    | [ H : _ |- _ ] => apply lem in H
-  end.
-
-Ltac apply_in_hyp_no_match lem :=
-  match goal with
-    | [ H : _ |- _ ] => apply lem in H;
-      match type of H with
-        | appcontext[match _ with _ => _ end] => fail 1
-        | _ => idtac
-      end
-  end.
-
-Ltac destruct_ex :=
-  repeat match goal with
-           | [ H : ex _ |- _ ] => destruct H; intuition
-         end.
-
-Hint Extern 0 => apply reflexivity : typeclass_instances.
-
-Ltac set_evars :=
-  repeat match goal with
-           | [ |- appcontext[?E] ] => is_evar E; let H := fresh in set (H := E)
-         end.
-
-Instance pointwise_refl A B (eqB : relation B) `{Reflexive _ eqB} : Reflexive (pointwise_relation A eqB).
-Proof.
-  compute in *; auto.
-Defined.
-
-Instance pointwise_sym A B (eqB : relation B) `{Symmetric _ eqB} : Symmetric (pointwise_relation A eqB).
-Proof.
-  compute in *; auto.
-Defined.
-
-Instance pointwise_transitive A B (eqB : relation B) `{Transitive _ eqB} : Transitive (pointwise_relation A eqB).
-Proof.
-  compute in *; eauto.
-Defined.
+Require Import Common.
 
 Section formulas.
   Inductive formula (vars : Type) :=
@@ -91,154 +41,6 @@ Section formulas.
          | Not x => Not (subst_vars bool_map x)
        end.
 End formulas.
-
-Section funcs.
-  Variable funcs : string -> Type * Type.
-  Inductive Comp : Type -> Type :=
-  | Return : forall A, A -> Comp A
-  | Bind : forall A B, Comp A -> (A -> Comp B) -> Comp B
-  | Call : forall x, fst (funcs x) -> Comp (snd (funcs x))
-  | Pick : forall A, Ensemble A -> Comp A.
-
-  Bind Scope comp_scope with Comp.
-  Global Arguments Bind A%type B%type _%comp _.
-
-  Notation "x >>= y" := (Bind x y) : comp_scope.
-  Notation "x <- y ; z" := (Bind y (fun x => z)) : comp_scope.
-  Notation "x ;; z" := (Bind x (fun _ => z)) : comp_scope.
-  Notation "f [[ x ]]" := (@Call f x) (at level 35) : comp_scope.
-  Notation "{ x  |  P }" := (@Pick _ (fun x => P)) : comp_scope.
-  Notation "{ x : A  |  P }" := (@Pick A (fun x => P)) : comp_scope.
-
-  Definition Or : Comp bool -> Comp bool -> Comp bool
-    := fun c1 c2 =>
-         (b1 <- c1;
-          if b1
-          then Return true
-          else c2)%comp.
-
-  Variable denote_funcs : forall name, fst (funcs name) -> Comp (snd (funcs name)).
-
-  Inductive computes_to
-  : forall A : Type, Comp A -> A -> Prop :=
-  | ReturnComputes : forall A v, @computes_to A (Return v) v
-  | BindComputes : forall A B comp_a f comp_a_value comp_b_value,
-                     @computes_to A comp_a comp_a_value
-                     -> @computes_to B (f comp_a_value) comp_b_value
-                     -> @computes_to B (Bind comp_a f) comp_b_value
-  | PickComputes : forall A (P : Ensemble A) v, P v -> @computes_to A (Pick P) v
-  | CallComputes : forall name (input : fst (funcs name)) (output_v : snd (funcs name)),
-                     @computes_to _ (denote_funcs name input) output_v
-                     -> @computes_to _ (Call name input) output_v.
-
-  Theorem computes_to_inv A (c : Comp A) v
-    : computes_to c v -> match c with
-                           | Return _ x => fun v => v = x
-                           | Bind _ _ x f => fun v => exists comp_a_value,
-                             computes_to x comp_a_value
-                             /\ computes_to (f comp_a_value) v
-                           | Call name input => computes_to (denote_funcs name input)
-                           | Pick _ P => P
-                         end v.
-  Proof.
-    destruct 1; eauto.
-  Qed.
-
-  (** The old program might be non-deterministic, and the new program
-      less so.  This means we want to say that if [new] can compute to
-      [v], then [old] should be able to compute to [v], too. *)
-  Definition refine {A} (old new : Comp A) := forall v, computes_to new v -> computes_to old v.
-
-  Global Instance refine_PreOrder A : PreOrder (@refine A).
-  Proof.
-    split; compute in *; eauto.
-  Qed.
-
-  Section monad.
-    Local Ltac t :=
-      split;
-      intro;
-      repeat match goal with
-               | [ H : _ |- _ ]
-                 => inversion H; clear H; subst; [];
-                    repeat match goal with
-                             | [ H : _ |- _ ] => apply inj_pair2 in H; subst
-                           end
-             end;
-      repeat first [ eassumption
-                   | solve [ constructor ]
-                   | eapply BindComputes; (eassumption || (try eassumption; [])) ].
-
-    Lemma bind_bind X Y Z (f : X -> Comp Y) (g : Y -> Comp Z) x v
-    : computes_to (Bind (Bind x f) g) v
-      <-> computes_to (Bind x (fun u => Bind (f u) g)) v.
-    Proof.
-      t.
-    Qed.
-
-    Lemma bind_unit X Y (f : X -> Comp Y) x v
-    : computes_to (Bind (Return x) f) v
-      <-> computes_to (f x) v.
-    Proof.
-      t.
-    Qed.
-
-    Lemma unit_bind X (x : Comp X) v
-    : computes_to (Bind x (@Return X)) v
-      <-> computes_to x v.
-    Proof.
-      t.
-    Qed.
-  End monad.
-End funcs.
-
-Hint Constructors computes_to.
-
-Notation "x >>= y" := (Bind x y) : comp_scope.
-Notation "x <- y ; z" := (Bind y (fun x => z)) : comp_scope.
-Notation "x ;; z" := (Bind x (fun _ => z)) : comp_scope.
-Notation "'call' f 'from' funcs [[ x ]]" := (@Call funcs f x) (at level 35) : comp_scope.
-Notation "{ x  |  P }" := (@Pick _ _ (fun x => P)) : comp_scope.
-Notation "{ x : A  |  P }" := (@Pick _ A (fun x => P)) : comp_scope.
-Notation ret := (Return _).
-
-Add Parametric Relation funcs denote_funcs A : (Comp funcs A) (@refine funcs denote_funcs A)
-  reflexivity proved by reflexivity
-  transitivity proved by transitivity
-    as refine_rel.
-
-Add Parametric Morphism funcs denote_funcs A B : (@Bind funcs A B)
-  with signature (@refine funcs denote_funcs A) ==> (pointwise_relation _ (@refine funcs denote_funcs B)) ==> (@refine funcs denote_funcs B)
-    as refine_bind.
-Proof.
-  intros.
-  unfold pointwise_relation, refine in *.
-  intros.
-  repeat (repeat apply_in_hyp_no_match computes_to_inv;
-    destruct_ex).
-  eauto.
-Qed.
-
-Section general_refine_lemmas.
-  Variable funcs : string -> Type * Type.
-  Variable denote_funcs : forall name, fst (funcs name) -> Comp funcs (snd (funcs name)).
-
-  Lemma refine_pick_pair A B (PA : A -> Prop) (PB : B -> Prop)
-  : refine denote_funcs
-           { x : A * B | PA (fst x) /\ PB (snd x) }%comp
-           (a <- { a : A | PA a };
-            b <- { b : B | PB b };
-            ret (a, b))%comp.
-  Proof.
-    intros (a, b) H.
-    repeat match goal with
-             | _ => constructor; tauto
-             | _ => progress destruct_ex
-             | [ H : (_, _) = (_, _) |- _ ] => inversion_clear H
-             | [ H : _ |- _ ] => apply computes_to_inv in H
-           end.
-  Qed.
-End general_refine_lemmas.
 
 Section op_funcs.
   Variable op : nat -> nat -> Prop.
@@ -397,15 +199,163 @@ Section min_max_funcs.
   Defined.
 End min_max_funcs.
 
+Section sort.
+  Variable T : Type.
+  Variable R : relation T.
+
+  Definition sort0 funcs (l : list T) : Comp funcs (list T)
+    := { l' : list T | Sorted R l' /\ Permutation l l' }%comp.
+
+  Variable pre_funcs : string -> Type * Type.
+
+  Definition funcs : string -> Type * Type
+    := (fun s =>
+          if string_dec s "sort"
+          then (list T, list T)
+          else pre_funcs s).
+
+  Definition sort1 (l : list T) : Comp funcs (list T)
+    := (x <- { x : T | List.In x l /\ Forall (R x) l };
+        xs <- { xs : list T | Permutation (x::xs) l };
+        xs' <- call "sort" from funcs [[ xs ]];
+        ret (x::xs'))%comp.
+
+  Definition sort2 (l : list T) : Comp funcs (list T)
+
+
 Section sat_funcs.
   Variable var : Type.
   Variable dec_eq : forall x y : var, {x = y} + {x <> y}.
+
+  Definition sat0 funcs (f : formula var) : Comp funcs bool
+    := { b : bool | b = true <-> is_satisfiable f }%comp.
 
   Definition funcs : string -> Type * Type
     := (fun s =>
       if string_dec s "sat"
       then (formula var, bool : Type)
       else (Datatypes.Empty_set : Type, unit : Type)).
+
+  Axiom sat1 : forall (f : formula var), Comp funcs bool.
+
+  Lemma sat_0_1 denote_funcs f : refine denote_funcs (sat0 funcs f) (sat1 f).
+  Proof.
+    unfold sat0.
+
+  Variable op : nat -> nat -> Prop.
+  Variable on_empty : nat -> Prop.
+  Definition is_op (l : list nat) (v : nat)
+    := Forall (fun n => op v n) l /\ (List.In v l \/ (l = nil /\ on_empty v)).
+
+  Variable funcs : string -> Type * Type.
+  Variable denote_funcs : forall name, fst (funcs name) -> Comp funcs (snd (funcs name)).
+
+  Definition is_op0 (l : list nat) : Comp funcs nat :=
+    { x : nat
+      | is_op l x }%comp.
+
+  Variable concrete_op : nat -> nat -> nat.
+  Variable concrete_on_empty : nat.
+  Hypothesis concrete_op_commutes : forall x y, concrete_op x y = concrete_op y x.
+  Hypothesis concrete_op_assoc : forall x y z, concrete_op (concrete_op x y) z = concrete_op x (concrete_op y z).
+  Hypothesis on_empty_concrete_on_empty : on_empty concrete_on_empty.
+  Hypothesis concrete_op_returns_arg : forall n m,
+    concrete_op n m = n \/ concrete_op n m = m.
+  Hypothesis concrete_op_preserves_op1 : forall n m,
+    op (concrete_op n m) m.
+  Hypothesis concrete_op_preserves_op2 : forall n m,
+    op (concrete_op n m) n.
+  Hypothesis op_refl : Reflexive op.
+  Hypothesis op_trans : Transitive op.
+
+  Definition is_op1 (l : list nat) : Comp funcs (nat : Type) :=
+    (ret (match l with
+            | nil => concrete_on_empty
+            | x::xs => fold_left concrete_op xs x
+          end))%comp.
+
+  Lemma fold_left_concrete_op_preserves_op l
+    : forall acc,
+      op (fold_left concrete_op l acc) acc.
+  Proof.
+    induction l; simpl; eauto.
+  Qed.
+
+  Hint Resolve fold_left_concrete_op_preserves_op.
+
+  Local Hint Constructors or.
+
+  Lemma fold_left_concrete_op_returns_in l
+    : forall acc,
+      acc = fold_left concrete_op l acc
+      \/ List.In (fold_left concrete_op l acc) l.
+  Proof.
+    induction l; simpl; eauto.
+    intro acc.
+    destruct (IHl acc) as [ IH1' | IH1' ];
+      try rewrite <- IH1';
+      edestruct concrete_op_returns_arg as [H|H];
+      erewrite H;
+      eauto.
+  Qed.
+
+  Hint Resolve fold_left_concrete_op_returns_in.
+
+  Lemma fold_left_concrete_op_commutes l
+  : forall a n, fold_left concrete_op l (concrete_op a n) = concrete_op (fold_left concrete_op l n) a.
+  Proof.
+    induction l; simpl; trivial.
+    intros.
+    rewrite <- IHl.
+    f_equal.
+    auto.
+  Qed.
+
+  Lemma op_works l
+  : Forall (fun n => match l with
+                       | [] => True
+                       | v::l => op (fold_left concrete_op l v) n
+                     end)
+           l.
+  Proof.
+    induction l; trivial.
+    constructor; [ apply fold_left_concrete_op_preserves_op | ].
+    destruct l; simpl in *; trivial.
+    inversion_clear IHl.
+    constructor;
+      eauto.
+    eapply Forall_impl; [ | eassumption ]; instantiate; simpl.
+    intros.
+    rewrite fold_left_concrete_op_commutes.
+    etransitivity; [ | eassumption ]; eauto.
+  Qed.
+
+  Theorem is_op_0_1
+    : pointwise_relation _ (refine denote_funcs) is_op0 is_op1.
+  Proof.
+    intros l v old_hyp.
+    unfold is_op1, is_op0 in *.
+    apply computes_to_inv in old_hyp.
+    subst.
+    constructor.
+    destruct l; simpl.
+    - hnf; simpl; intuition.
+    - split; [ | left; apply fold_left_concrete_op_returns_in ].
+      apply (op_works (_::_)).
+  Qed.
+
+  Theorem is_op_0_1' l
+    : refine denote_funcs
+             { x : nat
+             | is_op l x }%comp
+             (ret (match l with
+                     | nil => concrete_on_empty
+                     | x::xs => fold_left concrete_op xs x
+                   end))%comp.
+  Proof.
+    apply is_op_0_1.
+  Qed.
+
 
   Definition sat (f : formula var)
   : Comp funcs bool :=
