Common.v
@@ -1,0 +1,45 @@
+Require Export Setoid RelationClasses Program Morphisms.
+
+Global Set Implicit Arguments.
+Global Generalizable All Variables.
+
+Ltac apply_in_hyp lem :=
+  match goal with
+    | [ H : _ |- _ ] => apply lem in H
+  end.
+
+Ltac apply_in_hyp_no_match lem :=
+  match goal with
+    | [ H : _ |- _ ] => apply lem in H;
+      match type of H with
+        | appcontext[match _ with _ => _ end] => fail 1
+        | _ => idtac
+      end
+  end.
+
+Ltac destruct_ex :=
+  repeat match goal with
+           | [ H : ex _ |- _ ] => destruct H; intuition
+         end.
+
+Hint Extern 0 => apply reflexivity : typeclass_instances.
+
+Ltac set_evars :=
+  repeat match goal with
+           | [ |- appcontext[?E] ] => is_evar E; let H := fresh in set (H := E)
+         end.
+
+Instance pointwise_refl A B (eqB : relation B) `{Reflexive _ eqB} : Reflexive (pointwise_relation A eqB).
+Proof.
+  compute in *; auto.
+Defined.
+
+Instance pointwise_sym A B (eqB : relation B) `{Symmetric _ eqB} : Symmetric (pointwise_relation A eqB).
+Proof.
+  compute in *; auto.
+Defined.
+
+Instance pointwise_transitive A B (eqB : relation B) `{Transitive _ eqB} : Transitive (pointwise_relation A eqB).
+Proof.
+  compute in *; eauto.
+Defined.
