Computation.v
@@ -1,0 +1,158 @@
+Require Import String Ensembles.
+Require Import Common.
+
+Reserved Notation "x >>= y" (at level 42, right associativity).
+Reserved Notation "x <- y ; z" (at level 42, right associativity).
+Reserved Notation "x ;; z" (at level 42, right associativity).
+Reserved Notation "f [[ x ]]" (at level 35).
+Reserved Notation "'call' f 'from' funcs [[ x ]]" (at level 35).
+
+Delimit Scope comp_scope with comp.
+
+Section funcs.
+  Variable funcs : string -> Type * Type.
+  Inductive Comp : Type -> Type :=
+  | Return : forall A, A -> Comp A
+  | Bind : forall A B, Comp A -> (A -> Comp B) -> Comp B
+  | Call : forall x, fst (funcs x) -> Comp (snd (funcs x))
+  | Pick : forall A, Ensemble A -> Comp A.
+
+  Bind Scope comp_scope with Comp.
+  Global Arguments Bind A%type B%type _%comp _.
+
+  Notation "x >>= y" := (Bind x y) : comp_scope.
+  Notation "x <- y ; z" := (Bind y (fun x => z)) : comp_scope.
+  Notation "x ;; z" := (Bind x (fun _ => z)) : comp_scope.
+  Notation "f [[ x ]]" := (@Call f x) : comp_scope.
+  Notation "{ x  |  P }" := (@Pick _ (fun x => P)) : comp_scope.
+  Notation "{ x : A  |  P }" := (@Pick A (fun x => P)) : comp_scope.
+
+  Definition Or : Comp bool -> Comp bool -> Comp bool
+    := fun c1 c2 =>
+         (b1 <- c1;
+          if b1
+          then Return true
+          else c2)%comp.
+
+  Variable denote_funcs : forall name, fst (funcs name) -> Comp (snd (funcs name)).
+
+  Inductive computes_to
+  : forall A : Type, Comp A -> A -> Prop :=
+  | ReturnComputes : forall A v, @computes_to A (Return v) v
+  | BindComputes : forall A B comp_a f comp_a_value comp_b_value,
+                     @computes_to A comp_a comp_a_value
+                     -> @computes_to B (f comp_a_value) comp_b_value
+                     -> @computes_to B (Bind comp_a f) comp_b_value
+  | PickComputes : forall A (P : Ensemble A) v, P v -> @computes_to A (Pick P) v
+  | CallComputes : forall name (input : fst (funcs name)) (output_v : snd (funcs name)),
+                     @computes_to _ (denote_funcs name input) output_v
+                     -> @computes_to _ (Call name input) output_v.
+
+  Theorem computes_to_inv A (c : Comp A) v
+    : computes_to c v -> match c with
+                           | Return _ x => fun v => v = x
+                           | Bind _ _ x f => fun v => exists comp_a_value,
+                             computes_to x comp_a_value
+                             /\ computes_to (f comp_a_value) v
+                           | Call name input => computes_to (denote_funcs name input)
+                           | Pick _ P => P
+                         end v.
+  Proof.
+    destruct 1; eauto.
+  Qed.
+
+  (** The old program might be non-deterministic, and the new program
+      less so.  This means we want to say that if [new] can compute to
+      [v], then [old] should be able to compute to [v], too. *)
+  Definition refine {A} (old new : Comp A) := forall v, computes_to new v -> computes_to old v.
+
+  Global Instance refine_PreOrder A : PreOrder (@refine A).
+  Proof.
+    split; compute in *; eauto.
+  Qed.
+
+  Section monad.
+    Local Ltac t :=
+      split;
+      intro;
+      repeat match goal with
+               | [ H : _ |- _ ]
+                 => inversion H; clear H; subst; [];
+                    repeat match goal with
+                             | [ H : _ |- _ ] => apply inj_pair2 in H; subst
+                           end
+             end;
+      repeat first [ eassumption
+                   | solve [ constructor ]
+                   | eapply BindComputes; (eassumption || (try eassumption; [])) ].
+
+    Lemma bind_bind X Y Z (f : X -> Comp Y) (g : Y -> Comp Z) x v
+    : computes_to (Bind (Bind x f) g) v
+      <-> computes_to (Bind x (fun u => Bind (f u) g)) v.
+    Proof.
+      t.
+    Qed.
+
+    Lemma bind_unit X Y (f : X -> Comp Y) x v
+    : computes_to (Bind (Return x) f) v
+      <-> computes_to (f x) v.
+    Proof.
+      t.
+    Qed.
+
+    Lemma unit_bind X (x : Comp X) v
+    : computes_to (Bind x (@Return X)) v
+      <-> computes_to x v.
+    Proof.
+      t.
+    Qed.
+  End monad.
+End funcs.
+
+Hint Constructors computes_to.
+
+Notation "x >>= y" := (Bind x y) : comp_scope.
+Notation "x <- y ; z" := (Bind y (fun x => z)) : comp_scope.
+Notation "x ;; z" := (Bind x (fun _ => z)) : comp_scope.
+Notation "'call' f 'from' funcs [[ x ]]" := (@Call funcs f x) : comp_scope.
+Notation "{ x  |  P }" := (@Pick _ _ (fun x => P)) : comp_scope.
+Notation "{ x : A  |  P }" := (@Pick _ A (fun x => P)) : comp_scope.
+Notation ret := (Return _).
+
+Add Parametric Relation funcs denote_funcs A : (Comp funcs A) (@refine funcs denote_funcs A)
+  reflexivity proved by reflexivity
+  transitivity proved by transitivity
+    as refine_rel.
+
+Add Parametric Morphism funcs denote_funcs A B : (@Bind funcs A B)
+  with signature (@refine funcs denote_funcs A) ==> (pointwise_relation _ (@refine funcs denote_funcs B)) ==> (@refine funcs denote_funcs B)
+    as refine_bind.
+Proof.
+  intros.
+  unfold pointwise_relation, refine in *.
+  intros.
+  repeat (repeat apply_in_hyp_no_match computes_to_inv;
+    destruct_ex).
+  eauto.
+Qed.
+
+Section general_refine_lemmas.
+  Variable funcs : string -> Type * Type.
+  Variable denote_funcs : forall name, fst (funcs name) -> Comp funcs (snd (funcs name)).
+
+  Lemma refine_pick_pair A B (PA : A -> Prop) (PB : B -> Prop)
+  : refine denote_funcs
+           { x : A * B | PA (fst x) /\ PB (snd x) }%comp
+           (a <- { a : A | PA a };
+            b <- { b : B | PB b };
+            ret (a, b))%comp.
+  Proof.
+    intros (a, b) H.
+    repeat match goal with
+             | _ => constructor; tauto
+             | _ => progress destruct_ex
+             | [ H : (_, _) = (_, _) |- _ ] => inversion_clear H
+             | [ H : _ |- _ ] => apply computes_to_inv in H
+           end.
+  Qed.
+End general_refine_lemmas.
