Makefile
@@ -1,0 +1,56 @@
+MODULES    := \
+	Common \
+	Computation
+
+VS         := $(MODULES:%=%.v)
+VDS	   := $(MODULES:%=%.v.d)
+
+V = 0
+
+SILENCE_COQC_0 := @echo \"COQC $$<\"; #
+SILENCE_COQC_1 :=
+SILENCE_COQC = $(SILENCE_COQC_$(V))
+
+SILENCE_COQDEP_0 := @echo \"COQDEP $$<\"; #
+SILENCE_COQDEP_1 :=
+SILENCE_COQDEP = $(SILENCE_COQDEP_$(V))
+
+#NEW_TIME_FILE=time-of-build-after.log
+#OLD_TIME_FILE=time-of-build-before.log
+#BOTH_TIME_FILE=time-of-build-both.log
+#NEW_PRETTY_TIME_FILE=time-of-build-after-pretty.log
+#SINGLE_TIME_FILE=time-of-build.log
+#SINGLE_PRETTY_TIME_FILE=time-of-build-pretty.log
+#TIME_SHELF_NAME=time-of-build-shelf
+COQDOCFLAGS=-interpolate -utf8
+
+
+.PHONY: all html clean pretty-timed pretty-timed-files
+
+all: Makefile.coq
+	$(MAKE) -f Makefile.coq
+
+html: Makefile.coq
+	$(MAKE) -f Makefile.coq html
+
+#pretty-timed-diff:
+#	bash ./etc/make-each-time-file.sh "$(MAKE)" "$(NEW_TIME_FILE)" "$(OLD_TIME_FILE)"
+#	$(MAKE) combine-pretty-timed
+#
+#combine-pretty-timed:
+#	python ./etc/make-both-time-files.py "$(NEW_TIME_FILE)" "$(OLD_TIME_FILE)" "$(BOTH_TIME_FILE)"
+#	cat "$(BOTH_TIME_FILE)"
+#	@echo
+#
+#pretty-timed:
+#	bash ./etc/make-each-time-file.sh "$(MAKE) SEMICOLON=;" "$(SINGLE_TIME_FILE)"
+#	python ./etc/make-one-time-file.py "$(SINGLE_TIME_FILE)" "$(SINGLE_PRETTY_TIME_FILE)"
+#	cat "$(SINGLE_PRETTY_TIME_FILE)"
+#	@echo
+
+Makefile.coq: Makefile $(VS)
+	coq_makefile $(VS) -R . Synthesis COQC = " $(SILENCE_COQC)\$$(TIMER) \"\$$(COQBIN)coqc\"" COQDEP = " $(SILENCE_COQDEP)\"\$$(COQBIN)coqdep\" -c" COQDOCFLAGS = "$(COQDOCFLAGS)" -arg -dont-load-proofs -o Makefile.coq
+
+clean:: Makefile.coq
+	$(MAKE) -f Makefile.coq clean
+	rm -f Makefile.coq .depend
